testdata/out/go/completeslice_gk/completeslice_gk.go
@@ -10,40 +10,39 @@ import (
 )
 
 type S struct {
-	Strg string
-	Byte []byte
+	Strg  string
+	Bytes []byte
 }
 
-func (c *S) approxSize() uint64 {
-	return 0
-}
-
-func Marshal(c *S, prefix []byte) []byte {
+func Marshal(c S, prefix []byte) []byte {
 	var enc = prefix
 
 	strgBytes := []byte(c.Strg)
 	enc = marshal.WriteInt(enc, uint64(len(strgBytes)))
 	enc = marshal.WriteBytes(enc, strgBytes)
-	enc = marshal.WriteInt(enc, uint64(len(c.Byte)))
-	enc = marshal.WriteBytes(enc, c.Byte)
+	enc = marshal.WriteBytes(enc, c.Bytes)
 
 	return enc
 }
 
-func Unmarshal(s []byte) (*S, []byte) {
-	c := new(S)
+func Unmarshal(s []byte) (S, []byte) {
 	var enc = s // Needed for goose compatibility
+	var strg string
+	var bytes []byte
 
 	var strgLen uint64
 	var strgBytes []byte
 	strgLen, enc = marshal.ReadInt(enc)
 	strgBytes, enc = marshal.ReadBytesCopy(enc, strgLen)
-	c.Strg = string(strgBytes)
-	var byteLen uint64
-	var byteBytes []byte
-	byteLen, enc = marshal.ReadInt(enc)
-	byteBytes, enc = marshal.ReadBytesCopy(enc, byteLen)
-	c.Byte = byteBytes
+	strg = string(strgBytes)
+	var bytesLen uint64
+	var bytesBytes []byte
+	bytesLen, enc = marshal.ReadInt(enc)
+	bytesBytes, enc = marshal.ReadBytesCopy(enc, bytesLen)
+	bytes = bytesBytes
 
-	return c, enc
+	return S{
+		Strg:  strg,
+		Bytes: bytes,
+	}, enc
 }
