testdata/out/coq/completeslice_proof.v
@@ -3,6 +3,7 @@
 (*    DO NOT MANUALLY EDIT THIS FILE     *)
 (*****************************************)
 
+From Perennial.goose_lang.lib.list Require Import list.
 From Perennial.program_proof Require Import grove_prelude.
 From Perennial.program_proof Require Import marshal_stateless_proof.
 From Goose Require Import github_com.mjschwenne.grackle.testdata.out.go.completeslice_gk.
@@ -17,40 +18,95 @@ Context `{!heapGS Σ}.
 Record C :=
     mkC {
         strg : string;
-        byte : list u8;
+        bytes : list u8;
         }.
 
 Definition has_encoding (encoded:list u8) (args:C) : Prop :=
   encoded = (u64_le $ length $ string_to_bytes args.(strg)) ++ string_to_bytes args.(strg) ++
-              (u64_le $ length $ args.(byte)) ++ args.(byte).
+              (u64_le $ length $ args.(bytes)) ++ args.(bytes).
 
-Definition own (args_ptr: loc) (args: C) (dq: dfrac) : iProp Σ :=
-  ∃ (byte_sl : Slice.t), 
-  "Hargs_strg" ∷ args_ptr ↦[completeslice_gk.S :: "Strg"]{dq} #(str args.(strg)) ∗
-  "Hargs_byte" ∷ args_ptr ↦[completeslice_gk.S :: "Byte"]{dq} (slice_val byte_sl) ∗
-  "Hargs_byte_sl" ∷ own_slice_small byte_sl byteT dq args.(byte)
-  .
+Definition own (args__v: val) (args__c: C) (dq: dfrac) : iProp Σ :=
+  ∃ (bytes_sl : Slice.t), 
+  "%Hown_struct" ∷ ⌜ args__v = (#(str args__c.(strg)), (slice_val bytes_sl, #()))%V ⌝ ∗
+  "Hown_bytes" ∷ own_slice_small bytes_sl byteT dq args__c.(bytes).
 
-Lemma wp_Encode (args_ptr:loc) (args:C) (pre_sl:Slice.t) (prefix:list u8) (dq: dfrac):
+Definition to_val' (c : C) : val :=
+  (#(str c.(strg)), (val_of_list ((λ u : u8, #u) <$> c.(bytes)), #())).
+
+Fixpoint opt_list {A:Type} (l : list (option A)) : option (list A) :=
+  match l with
+  | nil => Some nil
+  | Some v :: l' => match opt_list l' with
+                   | Some l'' => Some (v :: l'')
+                   | None => None
+                   end
+  | None :: l' => None
+  end.
+
+Definition from_val' (v : val) : option C :=
+  match v with
+  | (#(LitString strg), (bytes, #()))%V =>
+      match list_from_val bytes with
+       | Some bytes =>
+           match opt_list ((fun v : val => match v with
+            | #(LitByte b) => Some b
+            | _ => None
+           end) <$> bytes) with
+                      | Some bytes => Some (mkC strg bytes)
+                      | None => None
+                      end
+       | None => None
+      end
+  | _ => None
+  end.
+
+#[global]
+Instance completeSlice_into_val : IntoVal C.
+Proof.
+  refine {|
+    to_val := to_val';
+    from_val := from_val';
+    IntoVal_def := (mkC "" [])
+  |}.
+  intros v. 
+  destruct v as [strg bytes]; done.
+Defined.
+
+#[global]
+Instance completeSlice_into_val_for_type : IntoValForType C (struct.t S).
+Proof. constructor; auto 10. Defined.
+
+Lemma own_to_val (v : val) (c : C) (dq : dfrac) :
+  own v c dq -∗ own v c dq ∗ ⌜ v = to_val c ⌝.
+Proof.
+  iIntros "%Hown_struct".
+  
+  iUnfold own.
+  iSplitL.
+  + iPureIntro. done.
+  + iPureIntro. done.
+Qed.
+
+Lemma wp_Encode (args__v : val) (args__c : C) (pre_sl : Slice.t) (prefix : list u8) (dq : dfrac):
   {{{
-        own args_ptr args dq ∗
+        own args__v args__c dq ∗
         own_slice pre_sl byteT (DfracOwn 1) prefix
   }}}
-    completeslice_gk.Marshal #args_ptr (slice_val pre_sl)
+    completeslice_gk.Marshal args__v (slice_val pre_sl)
   {{{
         enc enc_sl, RET (slice_val enc_sl);
-        ⌜has_encoding enc args⌝ ∗
-        own args_ptr args dq ∗
+        ⌜ has_encoding enc args__c ⌝ ∗
+        own args__v args__c dq ∗
         own_slice enc_sl byteT (DfracOwn 1) (prefix ++ enc)
   }}}.
 
 Proof.
-  iIntros (?) "H HΦ". iDestruct "H" as "[Hown Hsl]". iNamed "Hown".
+  iIntros (?) "[Hown Hsl] HΦ".
   wp_rec. wp_pures.
+  iUnfold own in "Hown". iNamed "Hown". rewrite Hown_struct.
   wp_apply (wp_ref_to); first by val_ty.
   iIntros (?) "Hptr". wp_pures.
 
-  wp_loadField.
   wp_apply wp_StringToBytes. iIntros (?) "Hargs_strg_enc". wp_pures.
   wp_apply (wp_slice_len).
   iDestruct (own_slice_sz with "Hargs_strg_enc") as "%Hargs_strg_sz".
@@ -59,46 +115,51 @@ Proof.
   wp_load. wp_apply (wp_WriteBytes with "[$Hsl $Hargs_strg_enc]").
   iIntros (?) "[Hsl _]". wp_store.
 
-  iDestruct (own_slice_small_sz with "Hargs_byte_sl") as "%Hargs_byte_sz".
+  iDestruct (own_slice_small_sz with "Hargs_bytes_sl") as "%Hargs_bytes_sz".
   wp_loadField. wp_apply wp_slice_len. wp_load.
   wp_apply (wp_WriteInt with "[$Hsl]"). iIntros (?) "Hsl". wp_store.
 
   wp_loadField. wp_load.
-  wp_apply (wp_WriteBytes with "[$Hsl $Hargs_byte_sl]").
-  iIntros (?) "[Hsl Hargs_byte_sl]". wp_store.
+  wp_apply (wp_WriteBytes with "[$Hsl $Hargs_bytes_sl]").
+  iIntros (?) "[Hsl Hargs_bytes_sl]". wp_store.
 
 
   wp_load. iApply "HΦ". iModIntro. rewrite -?app_assoc.
   iFrame. iPureIntro.
 
-  unfold has_encoding. 
+  unfold has_encoding. split.
+  {
+  
   rewrite ?string_bytes_length.
   rewrite Hargs_strg_sz.
-  rewrite Hargs_byte_sz.
+  rewrite Hargs_bytes_sz.
   rewrite ?w64_to_nat_id. exact.
 
 Qed.
 
-Lemma wp_Decode enc enc_sl (args: C) (suffix: list u8) (dq: dfrac):
+Lemma wp_Decode (enc : list u8) (enc_sl : Slice.t) (args__c : C) (suffix : list u8) (dq : dfrac):
   {{{
-        ⌜has_encoding enc args⌝ ∗
+        ⌜ has_encoding enc args__c ⌝ ∗
         own_slice_small enc_sl byteT dq (enc ++ suffix)
   }}}
     completeslice_gk.Unmarshal (slice_val enc_sl)
   {{{
-        args_ptr suff_sl, RET (#args_ptr, suff_sl); own args_ptr args (DfracOwn 1) ∗
-                                                    own_slice_small suff_sl byteT dq suffix
+        args__v suff_sl, RET (args__v, suff_sl);
+        own args__v args__c (DfracOwn 1) ∗
+        own_slice_small suff_sl byteT dq suffix
   }}}.
 
 Proof.
   iIntros (?) "[%Henc Hsl] HΦ". wp_rec.
-  wp_apply wp_allocStruct; first by val_ty.
-  iIntros (?) "Hstruct". wp_pures.
   wp_apply wp_ref_to; first done.
-  iIntros (?) "Hptr". wp_pures.
-  iDestruct (struct_fields_split with "Hstruct") as "HH".
-  iNamed "HH".
-
+  iIntros (l__s) "Hs". wp_pures.
+  
+  wp_apply wp_ref_of_zero; first done.
+  iIntros (l__strg) "Hstrg". wp_pures.
+  
+  wp_apply wp_ref_of_zero; first done.
+  iIntros (l__bytes) "Hbytes". wp_pures.
+  
   rewrite Henc. rewrite -?app_assoc.
 
   wp_apply wp_ref_of_zero; first done. iIntros (strgLen) "HstrgLen". wp_pures.
@@ -114,23 +175,25 @@ Proof.
   wp_pures. wp_store. wp_store. wp_load.
   iApply own_slice_to_small in "Hstrg'".
   wp_apply (wp_StringFromBytes with "[$Hstrg']"). iIntros "_".
-  wp_storeField.
+  wp_store.
 
   wp_apply wp_allocN; first done; first by val_ty.
-  iIntros (?) "HbyteLen". iApply array_singleton in "HbyteLen". wp_pures.
+  iIntros (?) "HbytesLen". iApply array_singleton in "HbytesLen". wp_pures.
   wp_apply wp_allocN; first done; first by val_ty.
-  iIntros (?) "Hbyte". iApply array_singleton in "Hbyte". wp_pures.
+  iIntros (?) "Hbytes". iApply array_singleton in "Hbytes". wp_pures.
   wp_load. wp_apply (wp_ReadInt with "[$Hsl]").
   iIntros (?) "Hsl". wp_pures. wp_store. wp_store. wp_load. wp_load.
 
-  iDestruct (own_slice_small_sz with "Hsl") as %Hbyte_sz.
+  iDestruct (own_slice_small_sz with "Hsl") as %Hbytes_sz.
   wp_apply (wp_ReadBytesCopy with "[$]").
-  { rewrite length_app in Hbyte_sz. word. }
-  iIntros (??) "[Hbyte' Hsl]". iApply own_slice_to_small in "Hbyte'".
+  { rewrite length_app in Hbytes_sz. word. }
+  iIntros (??) "[Hbytes' Hsl]". iApply own_slice_to_small in "Hbytes'".
 
   wp_pures. wp_store. wp_store. wp_load. wp_storeField.
 
-  wp_load. wp_pures. iApply "HΦ". iModIntro. rewrite ?string_to_bytes_to_string. iFrame.
+  wp_load. wp_load. wp_load.
+  wp_pures. iApply "HΦ". iModIntro. rewrite ?string_to_bytes_to_string. iFrame.
+  iPureIntro. reflexivity.
 Qed.
 
 End completeSlice.
